Change matching proofs to rely on matcher_invariant

MECMAR/props/Match.v
@@ -118,18 +118,38 @@ Module Correctness.
       length (MatchState.captures x) = RegExp.capturingGroupsCount rer /\
       List.Forall.Forall (MatchState.captures x) (CaptureRange.Valid str).
 
+    Definition remainingChars (x: MatchState) (dir: Direction): nat := match dir with
+    | forward => length (MatchState.input x) - Z.to_nat (MatchState.endIndex x)
+    | backward => Z.to_nat (MatchState.endIndex x)
+    end.
+
     Lemma change_captures: forall str rer input endIndex cap cap',
       length cap' = RegExp.capturingGroupsCount rer ->
       List.Forall.Forall cap' (CaptureRange.Valid str) ->
       Valid str rer (match_state input endIndex cap) ->
       Valid str rer (match_state input endIndex cap').
     Proof.
-      intros str rer input endIndex cap cap' H0 H1 [ OI_x [ IO_x V_cap ]]. 
+      intros str rer input endIndex cap cap' H0 H1 [ OI_x [ IO_x V_cap ]].
       unfold Valid. split_conjs; try assumption.
     Qed.
 
     Lemma self_input: forall str rer x, Valid str rer x -> Valid (MatchState.input x) rer x.
     Proof. intros ? ? ? (<-&?&?&?). unfold Valid; split_conjs; try assumption. reflexivity. Qed.
+
+    Lemma step: forall str rer x dir n, Valid str rer x ->
+      (0 <= n)%Z ->
+      (n <= remainingChars x dir)%Z ->
+      Valid (MatchState.input x) rer
+        (match_state str
+           (if dir == forward
+            then (MatchState.endIndex x + n)%Z
+            else (MatchState.endIndex x - n)%Z) (MatchState.captures x)).
+    Proof.
+      intros ? ? [ ] ? ? (<-&?&?&?) ? ?. unfold Valid,IteratorOn in *; cbn in *.
+      split_conjs; try assumption; try reflexivity.
+      all: destruct dir; cbn in *; try lia.
+    Qed.
+
     End main.
 
     (*  Normalizes all MatchStates by doing the following:
@@ -137,6 +157,7 @@ Module Correctness.
         - Then, if the MatchState is known to be on a particular string, eliminate the string introduced at the previous step. *)
     Ltac normalize := repeat
     (   CaptureRange.normalize
+    ||  unfold remainingChars
     ||  simpl (match_state _ _ _) in *
     ||  simpl (MatchState.input _) in *
     ||  simpl (MatchState.endIndex _) in *
@@ -180,7 +201,16 @@ Module Correctness.
           pose proof (List.Update.Nat.Batch.success_length _ _ _ _ H) as <-
         end).
 
-    Ltac solvers t := assumption || reflexivity || CaptureRange.solvers t (*|| (Zhelper; apply characterClass_successful_state_Valid; assumption)*).
+    Ltac solvers t := assumption || reflexivity || CaptureRange.solvers t
+      || lazymatch goal with
+          | [ H1: List.Forall.Forall ?ls (CaptureRange.Valid ?input),
+              H3: List.Update.Nat.One.update ?v ?ls _ = Success ?ls',
+              Eq: _ = Success ?v
+              |- List.Forall.Forall ?ls' (CaptureRange.Valid ?input) ] =>
+              apply List.Update.Nat.One.prop_preservation with (1 := H1) (3 := H3);
+              (* Goal: CaptureRange.Valid _ ?v *)
+              try solve [ focus § _ [] _ § auto destruct in Eq; injection Eq as <-; constructor; (assumption + lia) ]
+          end.
     (* Solves the current goal by 1. normalizing the states 2. leveraging assumptions and reflexivity *)
     Local Ltac solve_impl t := solve [ normalize; unfold OnInput, Valid; (solvers t || t) ].
 
@@ -264,6 +294,12 @@ Module Correctness.
     ||  rewrite <- (ignores_captures_l (List.empty)) in *
     ||  rewrite <- (ignores_captures_r (List.empty)) in *
     ||  lazymatch goal with
+        | [ H: progress forward _ _ |- _ ] => dependent destruction H
+        | [ H: directionalProgress forward _ _ |- _ ] => dependent destruction H
+        | [ H: progress backward _ _ |- _ ] => dependent destruction H
+        | [ H: directionalProgress backward _ _ |- _ ] => dependent destruction H
+        | [ |- progress forward _ _ ] => constructor; constructor
+        | [ |- progress backward _ _ ] => constructor; constructor
         | [ H: progress _ (?i [@ _ $ _]) (Success (Some (?i [@ _ $ _]))) |- _ ] => fail
         | [ H: progress _ (?i1 [@ _ $ _]) (Success (Some (?i2 [@ _ $ _]))) |- _ ] =>
           let Tmp := fresh in
@@ -291,787 +327,9 @@ Module Correctness.
     Ltac saturate := repeat (normalize; saturate_step); normalize; try solvers.
   End Progress.
 
-  (** Intermediate value: We say that Matcher _honores its continuation_ if 
-      its continuation must succeed on an input the matcher called it with in order for the matcher to itself succeed. *)
-  Module IntermediateValue. Section main.
+
+  Module MatcherInvariant. Section main.
     Context `{ci: CharacterInstance}.
-
-    Definition HonoresContinuation (m: Matcher) (dir: Direction) (rer: RegExp) := forall x c z,
-      (* For any valid state *)
-      MatchState.Valid (MatchState.input x) rer x ->
-      (* If the overall computation succeeded *)
-      m x c = Success (Some z) ->
-      (* There is an intermediate value y that was produced by m and then passed to c which then succeeded. *)
-      exists y, MatchState.Valid (MatchState.input x) rer y /\ progress dir x (Success (Some y)) /\ c y = Success (Some z).
-
-    (*  Automated tactic to find the intermediate value 
-        It will also try to prove the conditions on the intermediate value.
-      *)
-    Ltac search := unfold wrap_option,HonoresContinuation in *; subst; lazymatch goal with
-    | [ H: Success _ = Success _ |- _ ] => injection H; clear H; intros H; search
-    | [ H: ?c ?y = Success ?z |- exists x, MatchState.Valid _ _ _ /\ progress ?dir _ _ /\ ?c x = Success ?z ] =>
-      exists y; split_conjs;
-      [ assumption + ( unfold MatchState.Valid; split_conjs; try MatchState.solve )
-      | try solve [Progress.saturate]
-      | apply H ]
-    end.
-
-    Lemma repeatMatcher: forall fuel dir rer m min max greedy parenIndex parenCount,
-          HonoresContinuation m dir rer ->
-          HonoresContinuation (fun x c => repeatMatcher' m min max greedy x c parenIndex parenCount fuel) dir rer.
-    Proof.
-      (* The 'recursive' case (i.e. when min is not zero or the endIndex is different from last iteration) *)
-      assert (forall x z rer s c fuel dir m min max greedy parenIndex parenCount,
-        MatchState.Valid (MatchState.input x) rer x ->
-        List.Update.Nat.Batch.update None (MatchState.captures x) (List.Range.Nat.Bounds.range parenIndex (parenIndex + parenCount)) = Success s ->
-        HonoresContinuation m dir rer ->
-        (forall dir rer m min max greedy parenIndex parenCount,
-          HonoresContinuation m dir rer ->
-          HonoresContinuation (Definitions.RepeatMatcher.matcher m min max greedy parenIndex parenCount fuel) dir rer) ->
-        (m (match_state (MatchState.input x) (MatchState.endIndex x) s)
-          (Definitions.RepeatMatcher.continuation x c m min max greedy parenIndex parenCount fuel) = Success (Some z)) ->
-        exists y : MatchState,
-          MatchState.Valid (MatchState.input x) rer y /\ progress dir x (Success (Some y)) /\ c y = Success (Some z)
-      ) as Rec. {
-        intros x z rer s c fuel dir m min max greedy parenIndex parenCount Vx Ex_s HCm IH Eq_rec.
-        unfold HonoresContinuation in HCm, IH.
-        specialize IH with (1 := HCm).
-        focus § _ (_ _ []) _ § remember as d in Eq_rec.
-        specialize HCm with (2 := Eq_rec).
-        specialize (HCm ltac:(MatchState.solve)) as [ y0 [ Vy0 [ Pxy0 Eq_dy0 ]]].
-        rewrite -> Heqd in Eq_dy0. unfold Definitions.RepeatMatcher.continuation in Eq_dy0.
-        focus § _ [] _ § auto destruct in Eq_dy0.
-        specialize IH with (1 := (MatchState.self_input _ _ _ Vy0)) (2 := Eq_dy0) as [ y1 [ Vy1 [ Py0y1 Eq_cy1 ]]].
-        search.
-      }
-
-      induction fuel; [ discriminate | ].
-      cbn. intros dir rer m min max greedy parenIndex parenCount HCm x c z Vx H.
-      repeat rewrite Nat.add_sub in *.
-      focus § _ [] _ § auto destruct in H.
-      - search.
-      - eapply Rec; eassumption.
-      - search.
-      - eapply Rec; eassumption.
-      - injection H as [=->].
-        eapply Rec; eassumption.
-      - search.
-    Qed.
-
-    Lemma characterSetMatcher: forall rer A invert dir,
-          HonoresContinuation (characterSetMatcher rer A invert dir) dir rer.
-    Proof.
-      intros rer A invert dir x c z Vx Eq_z.
-      unfold characterSetMatcher in Eq_z. focus § _ [] _ § auto destruct in Eq_z.
-      boolean_simplifier.
-      search.
-      - Zhelper. MatchState.normalize. lia.
-      - apply Progress.step. lia.
-    Qed.
-
-    Lemma backreferenceMatcher: forall rer n dir,
-          HonoresContinuation (backreferenceMatcher rer n dir) dir rer.
-    Proof.
-      unfold HonoresContinuation. intros rer n dir x c z Vx Eq_z.
-      unfold backreferenceMatcher in Eq_z. focus § _ [] _ § auto destruct in Eq_z.
-      - search.
-      - search.
-        + destruct dir; MatchState.normalize; cbn in *; lia.
-        + apply Progress.step. MatchState.normalize. cbn in *. lia.
-    Qed.
-
-    Lemma compileSubPattern: forall r ctx rer dir m,
-      compileSubPattern r ctx rer dir = Success m ->
-      HonoresContinuation m dir rer.
-    Proof.
-      induction r; intros ctx rer dir m Eq_m x c z; cbn in Eq_m |- *;
-      focus § _ [] _ -> _ § auto destruct.
-      - injection Eq_m as <-. intros; search.
-      - injection Eq_m as <-. apply characterSetMatcher.
-      - injection Eq_m as <-. apply characterSetMatcher.
-      - destruct ae.
-        + focus § _ [] _ § auto destruct in Eq_m. injection Eq_m as <-.
-          apply backreferenceMatcher.
-        + destruct esc; focus § _ [] _ § auto destruct in Eq_m; injection Eq_m as <-; apply characterSetMatcher.
-        + destruct esc; focus § _ [] _ § auto destruct in Eq_m; injection Eq_m as <-; apply characterSetMatcher.
-        + focus § _ [] _ § auto destruct in Eq_m. injection Eq_m as <-.
-          apply backreferenceMatcher.
-      - focus § _ [] _ § auto destruct in Eq_m. injection Eq_m as <-.
-        apply characterSetMatcher.
-      - focus § _ [] _ § auto destruct in Eq_m. injection Eq_m as <-.
-        intros Vx Eq_z.
-        focus § _ [] _ § auto destruct in Eq_z.
-        + injection Eq_z as ->. apply IHr1 with (1 := AutoDest_); assumption.
-        + apply IHr2 with (1 := AutoDest_0); assumption.
-      - focus § _ [] _ § auto destruct in Eq_m. injection Eq_m as <-.
-        apply repeatMatcher. apply IHr with (1 := AutoDest_).
-      - intros Vx Eq_z.
-        unfold HonoresContinuation in IHr1,IHr2.
-        focus § _ [] _ § auto destruct in Eq_m; injection Eq_m as <-.
-        + specialize IHr1 with (1 := AutoDest_) (2 := Vx) (3 := Eq_z) as [y0 [Vy0 [Pxy0 Eq_y0]]].
-          specialize IHr2 with (1 := AutoDest_0) (2 := (MatchState.self_input _ _ _ Vy0)) (3 := Eq_y0) as [y1 [Vy1 [Pxy1 Eq_y1]]].
-          search.
-        + specialize IHr2 with (1 := AutoDest_0) (2 := Vx) (3 := Eq_z) as [y0 [Vy0 [Pxy0 Eq_y0]]].
-          specialize IHr1 with (1 := AutoDest_) (2 := (MatchState.self_input _ _ _ Vy0)) (3 := Eq_y0) as [y1 [Vy1 [Pxy1 Eq_y1]]].
-          search.
-      - intros Vx Eq_z.
-        unfold HonoresContinuation in IHr.
-        focus § _ [] _ § auto destruct in Eq_m; injection Eq_m as <-.
-        specialize IHr with (1 := AutoDest_) (2 := Vx) (3 := Eq_z) as [y [Vy [Pxy Eq_y]]].
-        focus § _ [] _ § auto destruct in Eq_y.
-        focus § _ [] _ § auto destruct in AutoDest_1. rewrite -> Nat.add_sub in AutoDest_1.
-        search.
-        MatchState.normalize.
-        refine (List.Update.Nat.One.prop_preservation _ _ _ _ _ VCF_captures_y _ AutoDest_1).
-        focus § _ [] _ § auto destruct in AutoDest_0; injection AutoDest_0 as <-; Zhelper; MatchState.normalize; rewrite -> ?EqDec.inversion_true in *; cbn in *; try lia.
-      - injection Eq_m as Eq_m. subst. intros Vx Eq_m.
-        focus § _ [] _ § auto destruct in Eq_m. search.
-      - injection Eq_m as Eq_m. subst. intros Vx Eq_m.
-        focus § _ [] _ § auto destruct in Eq_m. search.
-      - injection Eq_m as Eq_m. subst. intros Vx Eq_m.
-        focus § _ [] _ § auto destruct in Eq_m. search.
-      - injection Eq_m as Eq_m. subst. intros Vx Eq_m.
-        focus § _ [] _ § auto destruct in Eq_m. search.
-      - intros Vx Eq_z.
-        unfold HonoresContinuation in IHr.
-        focus § _ [] _ § auto destruct in Eq_m; injection Eq_m as <-.
-        focus § _ [] _ § auto destruct in Eq_z.
-        specialize IHr with (1 := AutoDest_) (2 := Vx) (3 := AutoDest_0) as [y [Vy [Pxy Eq_y]]].
-        search.
-      - intros Vx Eq_z.
-        focus § _ [] _ § auto destruct in Eq_m; injection Eq_m as <-.
-        focus § _ [] _ § auto destruct in Eq_z.
-        search.
-      - intros Vx Eq_z.
-        unfold HonoresContinuation in IHr.
-        focus § _ [] _ § auto destruct in Eq_m; injection Eq_m as <-.
-        focus § _ [] _ § auto destruct in Eq_z.
-        specialize IHr with (1 := AutoDest_) (2 := Vx) (3 := AutoDest_0) as [y [Vy [Pxy Eq_y]]].
-        search.
-      - intros Vx Eq_z.
-        focus § _ [] _ § auto destruct in Eq_m; injection Eq_m as <-.
-        focus § _ [] _ § auto destruct in Eq_z.
-        search.
-    Qed.
-  End main. End IntermediateValue.
-
-  Module Monotony.
-    Lemma compilePattern `{ci: CharacterInstance}: forall r rer input i m,
-      compilePattern r rer = Success m ->
-      progress forward (match_state input (Z.of_nat i) (List.repeat None (RegExp.capturingGroupsCount rer))) (m input i).
-    Proof.
-      intros r rer input i m H.
-      unfold compilePattern in *.
-      focus § _ [] _ § auto destruct in H. injection H as <-.
-      cbn. focus § _ _ _ [] § auto destruct.
-      - constructor.
-      - boolean_simplifier. spec_reflector PeanoNat.Nat.leb_spec0.
-        (* Assert that the start state is valid *)
-        focus § _ _ [] _ § do (fun x => assert (MatchState.Valid input rer x) as V_x). {
-          constructor.
-          + subst. MatchState.solve.
-          + subst. split_conjs.
-            * subst. cbn. constructor; lia.
-            * cbn. rewrite -> List.repeat_length. reflexivity.
-            * intros j v Indexed.
-              cbn in Indexed. apply List.Indexing.Nat.repeat in Indexed. subst.
-              constructor.
-        }
-        (* Eval program; most cases are trivial since they fail *)
-        (focus § _ _ _ [] § do (fun t => destruct t as [ [ z | ] | ] eqn:Eq_z)); try solve[ constructor ].
-        (* Use the intermediate value lemma to conclude *)
-        pose proof (IntermediateValue.compileSubPattern _ _ _ _ _ AutoDest_ _ _ _ V_x Eq_z) as [y [V_y [ P_xy <- ]]].
-        constructor.
-        + MatchState.solve.
-        + dependent destruction P_xy. assumption.
-    Qed.
-  End Monotony.
-
-  Module Safety. Section main.
-    Context `{ci: CharacterInstance}.
-
-    Definition SafeMatcher (m: Matcher) (dir: Direction) (rer: RegExp) := forall x c,
-      (* For any valid state *)
-      MatchState.Valid (MatchState.input x) rer x ->
-      (* If the overall computation runs out of fuel *)
-      m x c = match_assertion_failed ->
-      (* There is an intermediate value y that was produced by m and then passed to c which then ran out of fuel. *)
-      exists y, MatchState.Valid (MatchState.input x) rer y /\ progress dir x (Success (Some y)) /\ c y = match_assertion_failed.
-
-    Ltac search := lazymatch goal with
-    | [ H: Failure _ = match_assertion_failed |- _ ] => try rewrite -> H in *; clear H; search
-    | [ H: ?c ?y = match_assertion_failed |- exists x, MatchState.Valid _ _ x /\ progress ?dir _ _ /\ ?c x = match_assertion_failed ] =>
-      exists y; split_conjs;
-      [ try Progress.solve
-      | try solve [Progress.saturate]
-      | apply H ]
-    end.
-
-    Lemma repeatMatcher: forall dir m min max greedy parenIndex parenCount rer,
-      Captures.Valid rer parenIndex parenCount ->
-      SafeMatcher m dir rer ->
-      SafeMatcher (fun x c => repeatMatcher m min max greedy x c parenIndex parenCount) dir rer.
-    Proof.
-      assert (Ind: forall fuel dir m min max greedy parenIndex parenCount rer,
-        Captures.Valid rer parenIndex parenCount ->
-        SafeMatcher m dir rer ->
-        SafeMatcher (fun x c => repeatMatcher' m min max greedy x c parenIndex parenCount fuel) dir rer). {
-          induction fuel; intros dir m min max greedy parenIndex parenCount rer V_captures S_m x c V_x Eq_af; cbn in Eq_af; try easy.
-          focus § _ [] _ § auto destruct in Eq_af.
-          - search.
-          - apply S_m in Eq_af as [ y0 [ V_y0 [ P_x_y0 Eq_af ]]]; try MatchState.solve.
-            + focus § _ [] _ § auto destruct in Eq_af.
-              apply (IHfuel _ _ _ _ greedy parenIndex parenCount _ V_captures S_m _ c (MatchState.self_input _ _ _ V_y0)) in Eq_af as [ y1 [ V_y1 [ P_y0_y1 Eq_af ]]].
-              search.
-          - apply S_m in Eq_af as [ y0 [ V_y0 [ P_x_y0 Eq_af ]]]; try MatchState.solve.
-            focus § _ [] _ § auto destruct in Eq_af.
-            apply (IHfuel _ _ _ _ greedy parenIndex parenCount _ V_captures S_m _ c (MatchState.self_input _ _ _ V_y0)) in Eq_af as [ y1 [ V_y1 [ P_y0_y1 Eq_af ]]].
-            search.
-          - rewrite <- Eq_af. search.
-          - search.
-          - injection Eq_af as ->.
-            apply S_m in AutoDest_3 as [ y0 [ V_y0 [ P_x_y0 Eq_af ]]]; try MatchState.solve.
-            focus § _ [] _ § auto destruct in Eq_af.
-            apply (IHfuel _ _ _ _ greedy parenIndex parenCount _ V_captures S_m _ c (MatchState.self_input _ _ _ V_y0)) in Eq_af as [ y1 [ V_y1 [ P_y0_y1 Eq_af ]]].
-            search.
-          - injection Eq_af as ->.
-            apply List.Update.Nat.Batch.failure_bounds in AutoDest_0. unfold Captures.Valid in V_captures.
-            destruct V_x as [ _ [ _ [ VCL_x _ ]]]. rewrite -> VCL_x in *. repeat rewrite Nat.add_sub in *. contradiction.
-      }
-      intros dir m min max greedy parenIndex parenCount rer H H0 x c H1 H2. specialize Ind with (1 := H) (2 := H0).
-      unfold repeatMatcher. unfold SafeMatcher in Ind.
-      apply Ind with (1 := H1) (2 := H2).
-    Qed.
-
-    Lemma characterSetMatcher: forall rer A invert dir,
-      SafeMatcher (characterSetMatcher rer A invert dir) dir rer.
-    Proof.
-      intros rer A invert dir x c Vx Eq_oof.
-      unfold characterSetMatcher in Eq_oof. focus § _ [] _ § auto destruct in Eq_oof; hypotheses_reflector.
-      - search.
-        + Zhelper. MatchState.solve_with lia.
-        + apply Progress.step. lia.
-(*       - injection Eq_oof as <-. unfold CharSet.exist in AutoDest_2. apply List.Exists.failure_kind in AutoDest_2 as [_ [ c' [ _ Can_failure ]]].
-        rewrite_canonicalize. discriminate. *)
-(*       - rewrite_canonicalize. discriminate. *)
-      - injection Eq_oof as ->. boolean_simplifier. Zhelper.
-        destruct Vx as [ Eq_str [ [ ? ? ] _ ]].
-        destruct dir; cbn in *.
-        + assert (Z.min (MatchState.endIndex x) (MatchState.endIndex x + 1) = MatchState.endIndex x)%Z as Tmp by lia.
-          rewrite -> Tmp in *; clear Tmp.
-          apply List.Indexing.Int.failure_bounds in AutoDest_0 as [ ? | ? ]; lia.
-        + assert (Z.min (MatchState.endIndex x) (MatchState.endIndex x - 1) = MatchState.endIndex x - 1)%Z as Tmp by lia.
-          rewrite -> Tmp in *; clear Tmp.
-          apply List.Indexing.Int.failure_bounds in AutoDest_0 as [ ? | ? ]; try lia.
-    Qed.
-
-    Lemma positiveLookaroundMatcher: forall m rer dir dir',
-      IntermediateValue.HonoresContinuation m dir' rer ->
-      SafeMatcher m dir' rer ->
-      SafeMatcher (Definitions.PositiveLookaround.matcher m) dir rer.
-    Proof.
-      intros m rer dir dir' HC_m S_m. intros x c V_x Eq_af.
-      unfold Definitions.PositiveLookaround.matcher in *.
-      focus § _ [] _ § auto destruct in Eq_af.
-      + specialize (HC_m _ _ _ V_x AutoDest_) as [ y0 [ V_y0 [ P_x_y0 [=<-] ]]].
-        search.
-      + injection Eq_af as ->.
-        specialize (S_m _ _ V_x AutoDest_) as [ y0 [ V_y0 [ P_x_y0 Eq_y0 ]]].
-        discriminate.
-    Qed.
-
-    Lemma negativeLookaroundMatcher: forall m rer dir dir',
-      SafeMatcher m dir' rer ->
-      SafeMatcher (Definitions.NegativeLookaround.matcher m) dir rer.
-    Proof.
-      intros m rer dir dir' S_m. intros x c V_x Eq_af.
-      unfold Definitions.NegativeLookaround.matcher in *.
-      focus § _ [] _ § auto destruct in Eq_af.
-      + search.
-      + injection Eq_af as ->.
-        specialize (S_m _ _ V_x AutoDest_) as [ y0 [ V_y0 [ P_x_y0 Eq_y0 ]]].
-        discriminate.
-    Qed.
-
-    Lemma backreferenceMatcher: forall rer n dir,
-      (positive_to_non_neg n) <= RegExp.capturingGroupsCount rer ->
-      SafeMatcher (backreferenceMatcher rer n dir) dir rer.
-    Proof.
-      intros rer n dir Bound_n x c Vx Eq_af.
-      unfold backreferenceMatcher in Eq_af. focus § _ [] _ § auto destruct in Eq_af.
-      - search.
-      - search.
-        + destruct dir; cbn in *; MatchState.solve_with ltac:(cbn in *; lia).
-        + apply Progress.step. MatchState.normalize. cbn in *. lia.
-      - injection Eq_af as ->. Zhelper.
-        apply List.Exists.failure_kind in AutoDest_3.
-        destruct AutoDest_3 as [ i [ j [ Eq_indexed Eq_af ]]].
-        pose proof Eq_indexed as Tmp. apply List.Range.Int.Bounds.indexing in Tmp as ->.
-        apply List.Indexing.Int.success_bounds in Eq_indexed as Bounds_i. clear Eq_indexed.
-        destruct Vx as [ Eq_str [ [ ? ? ] [ _ V_t ]]].
-        cbn in AutoDest_. focus § _ [] _ § auto destruct in AutoDest_.
-        specialize (V_t _ _ AutoDest_). dependent destruction V_t.
-        rename s into t_s, e into t_e, H into Ineq_t, H0 into IO_t_s, H1 into IO_t_e.
-        MatchState.normalize. cbn in *. rewrite -> List.Range.Int.Bounds.length in *.
-        focus § _ [] _ § auto destruct in Eq_af; injection Eq_af as ->.
-(*         + rewrite_canonicalize. discriminate. *)
-        + destruct dir; cbn in *.
-          * apply List.Indexing.Int.failure_bounds in AutoDest_1 as [ ? | ? ]; lia.
-          * apply List.Indexing.Int.failure_bounds in AutoDest_1 as [ ? | ? ]; lia.
-(*         + rewrite_canonicalize. discriminate. *)
-        + destruct dir.
-          * apply List.Indexing.Int.failure_bounds in AutoDest_0 as [ ? | ? ]; lia.
-          * apply List.Indexing.Int.failure_bounds in AutoDest_0 as [ ? | ? ]; lia.
-      - injection Eq_af as ->.
-        cbn in AutoDest_. focus § _ [] _ § auto destruct in AutoDest_.
-        apply List.Indexing.Nat.failure_bounds in AutoDest_.
-        destruct Vx as [ _ [ _ [ Tmp _ ]]]; rewrite -> Tmp in *; clear Tmp.
-        pose proof (NonNegInt.pos n). lia.
-    Qed.
-
-    Lemma compileSubPattern: forall rer root r ctx dir m,
-      countLeftCapturingParensWithin root nil = RegExp.capturingGroupsCount rer ->
-      Root root r ctx ->
-      EarlyErrors.Pass_Regex root nil ->
-      compileSubPattern r ctx rer dir = Success m ->
-      SafeMatcher m dir rer.
-    Proof.
-      intros rer root.
-      induction r; cbn; intros ctx dir m Eq_rer R_r GR_root Eq_m.
-      - focus § _ [] _ § auto destruct in Eq_m; injection Eq_m as <-.
-        intros x c Vx Sc. search.
-      - focus § _ [] _ § auto destruct in Eq_m; injection Eq_m as <-.
-        apply characterSetMatcher.
-      - focus § _ [] _ § auto destruct in Eq_m; injection Eq_m as <-.
-        apply characterSetMatcher.
-      - destruct ae.
-        + focus § _ [] _ § auto destruct in Eq_m; injection Eq_m as <-.
-          apply backreferenceMatcher. boolean_simplifier. spec_reflector Nat.leb_spec0. assumption.
-        + destruct esc; focus § _ [] _ § auto destruct in Eq_m; injection Eq_m as <-; apply characterSetMatcher.
-        + destruct esc; focus § _ [] _ § auto destruct in Eq_m; injection Eq_m as <-; apply characterSetMatcher.
-        + focus § _ [] _ § auto destruct in Eq_m; injection Eq_m as <-.
-          apply backreferenceMatcher. boolean_simplifier. cbn in *.
-          apply List.Unique.success in AutoDest_0. destruct s. cbn in *.
-          assert (List.Indexing.Nat.indexing (groupSpecifiersThatMatch (AtomEsc (GroupEsc id)) ctx id) 0 = Success (r, l)) as Eq_indexed. {
-            rewrite -> AutoDest_0. reflexivity.
-          }
-          pose proof (EarlyErrors.groupSpecifiersThatMatch_is_filter_map (AtomEsc (GroupEsc id)) ctx id) as (f & _ & Def_f).
-          apply Def_f in Eq_indexed. destruct Eq_indexed as (ctx' & ? & Eq_indexed).
-          subst. destruct (countLeftCapturingParensBefore_impl ctx' + 1) eqn:Eq; try lia. cbn in *.
-          apply Zipper.Walk.soundness in Eq_indexed. eapply Zipper.Down.same_root_down in Eq_indexed; [ | eapply R_r ]. cbn in *.
-          pose proof (EarlyErrors.countLeftCapturingParensBefore_contextualized _ _ _ Eq_indexed GR_root).
-          subst. unfold countLeftCapturingParensBefore,countLeftCapturingParensWithin in *. cbn in *.
-          apply NonNegInt.to_positive_soundness in AutoDest_1.
-          lia.
-      - focus § _ [] _ § auto destruct in Eq_m; injection Eq_m as <-.
-        apply characterSetMatcher.
-      - intros x c Vx Sc.
-        focus § _ [] _ § auto destruct in Eq_m; injection Eq_m as <-.
-        focus § _ [] _ § auto destruct in Sc.
-        + specialize (IHr2 (Disjunction_right r1 :: ctx) _ _ ltac:(eassumption) ltac:(eassumption) ltac:(eassumption) ltac:(eassumption) x c ltac:(eassumption) ltac:(eassumption)) as [ ? [ ? [ ? ? ]]].
-          search.
-        + injection Sc as ->.
-          specialize (IHr1 (Disjunction_left r2 :: ctx) _ _ ltac:(eassumption) ltac:(eassumption) ltac:(eassumption) ltac:(eassumption) x c ltac:(eassumption) ltac:(eassumption)) as [ ? [ ? [ ? ? ]]].
-          search.
-      - focus § _ [] _ § auto destruct in Eq_m; injection Eq_m as <-.
-        apply repeatMatcher.
-        + intros i v Eq_indexed.
-          pose proof (List.Indexing.Nat.success_bounds _ _ _ Eq_indexed). rewrite -> List.Range.Nat.Bounds.length in *.
-          apply List.Range.Nat.Bounds.indexing in Eq_indexed.
-          pose proof (EarlyErrors.countLeftCapturingParensBefore_contextualized _ _ _ R_r GR_root).
-          unfold countLeftCapturingParensBefore,countLeftCapturingParensWithin in *. cbn in *. lia.
-        + apply (IHr (Quantified_inner q :: ctx) _ _ ltac:(eassumption) ltac:(eassumption) ltac:(eassumption) ltac:(eassumption)).
-      - intros x c V_x S_c.
-        focus § _ [] _ § auto destruct in Eq_m; injection Eq_m as <-.
-        + specialize (IHr1 _ _ _ ltac:(eassumption) ltac:(eapply Zipper.Down.same_root_down0; [ constructor | eassumption]) ltac:(eassumption) ltac:(eassumption) _ _ V_x S_c) as [ y0 [ V_y0 [ P_x_y0 Eq_y0 ]]].
-          specialize (IHr2 _ _ _ ltac:(eassumption) ltac:(eapply Zipper.Down.same_root_down0; [ constructor | eassumption]) ltac:(eassumption) ltac:(eassumption) _ _ (MatchState.self_input _ _ _ V_y0) Eq_y0) as [ y1 [ V_y1 [ P_x_y1 Eq_y1 ]]].
-          search.
-        + specialize (IHr2 _ _ _ ltac:(eassumption) ltac:(eapply Zipper.Down.same_root_down0; [ constructor | eassumption]) ltac:(eassumption) ltac:(eassumption) _ _ V_x S_c) as [ y0 [ V_y0 [ P_x_y0 Eq_y0 ]]].
-          specialize (IHr1 _ _ _ ltac:(eassumption) ltac:(eapply Zipper.Down.same_root_down0; [ constructor | eassumption]) ltac:(eassumption) ltac:(eassumption) _ _ (MatchState.self_input _ _ _ V_y0) Eq_y0) as [ y1 [ V_y1 [ P_x_y1 Eq_y1 ]]].
-          search.
-      - intros x c V_x Eq_af.
-        focus § _ [] _ § auto destruct in Eq_m; injection Eq_m as <-.
-        specialize (IHr _ _ _ ltac:(eassumption) ltac:(eapply Zipper.Down.same_root_down0; [ constructor | eassumption]) ltac:(eassumption) ltac:(eassumption) _ _ V_x Eq_af) as [ y0 [ V_y0 [ P_x_y0 Eq_y0 ]]].
-        focus § _ [] _ § auto destruct in Eq_y0.
-        + focus § _ [] _ § auto destruct in AutoDest_0; focus § _ [] _ § auto destruct in AutoDest_1; rewrite -> Nat.add_sub in AutoDest_1.
-          * search. MatchState.solve_with lia.
-          * search. MatchState.solve_with lia.
-        + injection Eq_y0 as ->.
-          focus § _ [] _ § auto destruct in AutoDest_1.
-          * spec_reflector Nat.eqb_spec. lia.
-          * rewrite -> Nat.add_sub in *.
-            apply List.Update.Nat.One.failure_bounds in AutoDest_1.
-            pose proof (EarlyErrors.countLeftCapturingParensBefore_contextualized _ _ _ R_r GR_root).
-            unfold countLeftCapturingParensBefore,countLeftCapturingParensWithin in *. cbn in *. MatchState.solve_with lia.
-        + injection Eq_y0 as ->.
-          focus § _ [] _ § auto destruct in AutoDest_0; destruct dir; try discriminate.
-          * Zhelper. MatchState.normalize.
-            dependent destruction P_x_y0.
-            dependent destruction H0. cbn in *.
-            lia.
-          * Zhelper.
-            dependent destruction P_x_y0.
-            dependent destruction H0. cbn in *.
-            lia.
-      - injection Eq_m as Eq_m. subst. intros x c V_x Eq_af.
-        focus § _ [] _ § auto destruct in Eq_af; [search | injection Eq_af as <-].
-        focus § _ [] _ § auto destruct in AutoDest_.
-        + lazymatch goal with | [ H: List.Indexing.Int.indexing _ _ = Failure _ |- _ ] => apply List.Indexing.Int.failure_bounds in H end.
-          MatchState.solve_with lia.
-        + destruct (RegExp.multiline rer); discriminate.
-      - injection Eq_m as Eq_m. subst. intros x c V_x Eq_af.
-        focus § _ [] _ § auto destruct in Eq_af; [search | injection Eq_af as <-].
-        focus § _ [] _ § auto destruct in AutoDest_.
-        + match goal with | [ H: List.Indexing.Int.indexing _ _ = Failure _ |- _ ] => apply List.Indexing.Int.failure_bounds in H (*; MatchState.solve_with lia*) end.
-          MatchState.solve_with lia.
-        + destruct (RegExp.multiline rer); discriminate.
-      - injection Eq_m as Eq_m. subst. intros x c V_x Eq_af.
-        focus § _ [] _ § auto destruct in Eq_af; try search.
-        all: lazymatch goal with | [ H: isWordChar _ _ _ = Failure _ |- _ ] =>  unfold isWordChar in H; focus § _ [] _ § auto destruct in H; clear_result; subst end.
-        all: try lazymatch goal with
-            | [ H: wordCharacters _ = Failure _ |- _ ] => exfalso; apply (Compile.wordCharacters _ _ H)
-            | [ H: _ [_] = Failure _ |- _ ] => apply List.Indexing.Int.failure_bounds in H; MatchState.solve_with lia
-            end.
-      - injection Eq_m as Eq_m. subst. intros x c V_x Eq_af.
-        focus § _ [] _ § auto destruct in Eq_af; try search.
-        all: lazymatch goal with | [ H: isWordChar _ _ _ = Failure _ |- _ ] =>  unfold isWordChar in H; focus § _ [] _ § auto destruct in H; clear_result; subst end.
-        all: try lazymatch goal with
-            | [ H: wordCharacters _ = Failure _ |- _ ] => exfalso; apply (Compile.wordCharacters _ _ H)
-            | [ H: _ [_] = Failure _ |- _ ] => apply List.Indexing.Int.failure_bounds in H; MatchState.solve_with lia
-            end.
-      - focus § _ [] _ § auto destruct in Eq_m; injection Eq_m as <-.
-        apply positiveLookaroundMatcher with (dir' := forward).
-        + apply IntermediateValue.compileSubPattern with (1 := AutoDest_).
-        + apply (IHr (Lookahead_inner :: ctx) _ _ ltac:(eassumption) ltac:(eassumption) ltac:(eassumption) ltac:(eassumption)).
-      - focus § _ [] _ § auto destruct in Eq_m; injection Eq_m as <-.
-        apply negativeLookaroundMatcher with (dir' := forward).
-        apply (IHr (NegativeLookahead_inner :: ctx) _ _ ltac:(eassumption) ltac:(eassumption) ltac:(eassumption) ltac:(eassumption)).
-      - focus § _ [] _ § auto destruct in Eq_m; injection Eq_m as <-.
-        apply positiveLookaroundMatcher with (dir' := backward).
-        + apply IntermediateValue.compileSubPattern with (1 := AutoDest_).
-        + apply (IHr (Lookbehind_inner :: ctx) _ _ ltac:(eassumption) ltac:(eassumption) ltac:(eassumption) ltac:(eassumption)).
-      - focus § _ [] _ § auto destruct in Eq_m; injection Eq_m as <-.
-        apply negativeLookaroundMatcher with (dir' := backward).
-        eapply (IHr (NegativeLookbehind_inner :: ctx) _ _ ltac:(eassumption) ltac:(eassumption) ltac:(eassumption) ltac:(eassumption)).
-    Qed.
-
-    Theorem compilePattern: forall r rer input i m,
-      EarlyErrors.Pass_Regex r nil ->
-      countLeftCapturingParensWithin r nil = RegExp.capturingGroupsCount rer ->
-      0 <= i <= (length input) ->
-      compilePattern r rer = Success m ->
-      m input i <> match_assertion_failed.
-    Proof.
-      intros r rer input i m GR Eq_rer Bounds_i Eq_m. unfold compilePattern in Eq_m. 
-      focus § _ [] _ § auto destruct in Eq_m. injection Eq_m as <-.
-      focus § _ (_ [] _) § auto destruct.
-      - hypotheses_reflector. spec_reflector Nat.leb_spec0. contradiction.
-      - remember (match_state input i (List.repeat None (RegExp.capturingGroupsCount rer))) as x eqn:Eq_x.
-        pose proof (compileSubPattern _ _ _ nil forward _ Eq_rer (Zipper.Root.id _) GR AutoDest_ x (fun y => y)) as Falsum.
-        assert (MatchState.Valid (MatchState.input x) rer x) as V_x. {
-          subst x. apply MatchState.valid_init. lia.
-        }
-        focus § _ (_ [] _) § do (fun t => destruct t as [ | f ]; try easy; destruct f; try easy).
-        fforward Falsum. destruct Falsum as [ ? [ _ [ _ ? ]]].
-        subst. discriminate.
-    Qed.
-  End main. End Safety.
-
-  Module Termination. Section main.
-    Context `{ci: CharacterInstance}.
-    Definition TerminatingMatcher (m: Matcher) (dir: Direction) (rer: RegExp) := forall x c,
-      (* For any valid state *)
-      MatchState.Valid (MatchState.input x) rer x ->
-      (* If the overall computation runs out of fuel *)
-      m x c = out_of_fuel ->
-      (* There is an intermediate value y that was produced by m and then passed to c which then ran out of fuel. *)
-      exists y, MatchState.Valid (MatchState.input x) rer y /\ progress dir x (Success (Some y)) /\ c y = out_of_fuel.
-
-    Definition remainingChars (x: MatchState) (dir: Direction): nat := match dir with
-    | forward => length (MatchState.input x) - Z.to_nat (MatchState.endIndex x)
-    | backward => Z.to_nat (MatchState.endIndex x)
-    end.
-    Definition fuelBound (min: non_neg_integer) (x: MatchState) (dir: Direction) := min + (remainingChars x dir)  + 1.
-
-    Lemma repeatMatcherFuel_satisfies_bound: forall min x rer dir, MatchState.Valid (MatchState.input x) rer x -> fuelBound min x dir <= repeatMatcherFuel min x.
-    Proof. intros. unfold fuelBound,repeatMatcherFuel in *. destruct H as [ ? [ [ Bounds_Ei_x_low Bounds_Ei_x_high ] VC_x ] ]. destruct dir; cbn; lia. Qed.
-
-    Lemma fuelDecreases_min: forall dir min min' x x' b,
-      min' < min -> progress dir x (Success (Some x')) -> fuelBound min x dir <= S b -> fuelBound min' x' dir <= b.
-    Proof.
-      intros. unfold fuelBound,remainingChars in *. inversion H0; destruct dir; inversion H6; subst.
-      - rewrite -> H3 in *. lia.
-      - lia.
-    Qed.
-
-    Lemma fuelDecreases_progress: forall dir rer min x x' b,
-      progress dir x (Success (Some x')) ->
-      ((MatchState.endIndex x) =? (MatchState.endIndex x'))%Z = false ->
-      MatchState.Valid (MatchState.input x) rer x ->
-      MatchState.Valid (MatchState.input x) rer x' ->
-      fuelBound min x dir <= S b ->
-      fuelBound min x' dir <= b.
-    Proof.
-      intros dir rer min x x' b P_x_x' Neq_Eis [ ? [ [ Bei_x_l Bei_x_h ] VC_x ] ] [ ? [ [ B_Ei_x'_l B_Ei_x'_h ] VC_x' ] ] Ineq_fuel.
-      dependent destruction P_x_x'. rename H into Eq_inp_x_x', H0 into Dp_x_x'.
-      unfold fuelBound, remainingChars in *.
-      rewrite <- Eq_inp_x_x' in *.
-      spec_reflector Z.eqb_spec.
-      dependent destruction Dp_x_x'; lia.
-    Qed.
-
-    Ltac search := lazymatch goal with
-    | [ H: Failure _ = out_of_fuel |- _ ] => try rewrite -> H in *; clear H; search
-    | [ H: ?c ?y = out_of_fuel |- exists x, MatchState.Valid _ _ x /\ progress ?dir _ _ /\ ?c x = out_of_fuel ] =>
-      exists y; split; [ | split ];
-      [ try Progress.solve
-      | try solve [Progress.saturate]
-      | apply H ]
-    end.
-
-    Lemma repeatMatcher': forall fuel m min max greedy parenIndex parenCount x c dir rer,
-      fuelBound min x dir <= fuel ->
-      MatchState.Valid (MatchState.input x) rer x ->
-      TerminatingMatcher m dir rer ->
-      repeatMatcher' m min max greedy x c parenIndex parenCount fuel = out_of_fuel ->
-      exists y,
-        MatchState.Valid (MatchState.input x) rer y /\ progress dir x (Success (Some y)) /\ c y = out_of_fuel.
-    Proof.
-      induction fuel; intros m min max greedy parenIndex parenCount x c dir rer Ineq_fuel Vx Tm Falsum.
-      - clear -Ineq_fuel. unfold fuelBound, remainingChars in *. lia.
-      - cbn in Falsum.
-        (focus § _ [] _ § auto destruct in Falsum).
-        + search.
-        + apply Tm in Falsum; try Progress.solve. destruct Falsum as [ y [ Vy [ Pxy Falsum ] ] ].
-          (focus § _ [] _ § auto destruct in Falsum). boolean_simplifier.
-          assert(FD: fuelBound (min - 1) y dir <= fuel). {
-            apply fuelDecreases_min with (min := min) (x := x); try Progress.solve.
-            spec_reflector Nat.eqb_spec. lia.
-          }
-          specialize IHfuel with (1 := FD) (2 := (MatchState.self_input _ _ _ Vy)) (3 := Tm) (4 := Falsum). clear Falsum.
-          destruct IHfuel as [ z [ Vz [ Pyz Falsum ] ] ].
-          search.
-        + apply Tm in Falsum; try Progress.solve. destruct Falsum as [ y [ Vy [ Pxy Falsum ] ] ].
-          (focus § _ [] _ § auto destruct in Falsum).
-          boolean_simplifier. spec_reflector Nat.eqb_spec. subst.
-          assert(FD: fuelBound 0 y dir <= fuel). {
-            (focus § _ [] _ § do (fun t => apply fuelDecreases_progress with (rer := rer) (x := t)) in Pxy); try Progress.solve.
-            MatchState.normalize. spec_reflector Z.eqb_spec. congruence.
-          }
-          specialize IHfuel with (1 := FD) (2 := (MatchState.self_input _ _ _ Vy)) (3 := Tm) (4 := Falsum). clear Falsum.
-          destruct IHfuel as [ z [ Vz [ Pyz Falsum ] ] ].
-          search.
-        + search.
-        + search.
-        + rewrite -> Falsum in *. clear Falsum. apply Tm in AutoDest_3; try Progress.solve. destruct AutoDest_3 as [ y [ Vy [ Pxy Falsum ] ] ].
-          (focus § _ [] _ § auto destruct in Falsum).
-          boolean_simplifier. spec_reflector Nat.eqb_spec. subst.
-          assert(FD: fuelBound 0 y dir <= fuel). {
-            (focus § _ [] _ § do (fun t => apply fuelDecreases_progress with (rer := rer) (x := t)) in Pxy); try Progress.solve.
-            MatchState.normalize. spec_reflector Z.eqb_spec. congruence.
-          }
-          specialize IHfuel with (1 := FD) (2 := (MatchState.self_input _ _ _ Vy)) (3 := Tm) (4 := Falsum). clear Falsum.
-          destruct IHfuel as [ z [ Vz [ Pyz Falsum ] ] ].
-          search.
-        + injection Falsum as ->.
-          apply List.Update.Nat.Batch.failure_is_assertion in AutoDest_0.
-          discriminate.
-    Qed.
-
-    Lemma repeatMatcher: forall m min max greedy parenIndex parenCount rer dir,
-      TerminatingMatcher m dir rer ->
-      TerminatingMatcher (fun x c => repeatMatcher m min max greedy x c parenIndex parenCount) dir rer.
-    Proof.
-      unfold Semantics.repeatMatcher, TerminatingMatcher. intros m min max greedy parenIndex parenCount rer dir Tm x c V_x Eq_oof.
-      apply repeatMatcher' with (4 := Eq_oof); try easy.
-      apply repeatMatcherFuel_satisfies_bound with (rer := rer).
-      assumption.
-    Qed.
-
-    Lemma characterSetMatcher: forall rer A invert dir,
-      TerminatingMatcher (characterSetMatcher rer A invert dir) dir rer.
-    Proof.
-      intros rer A invert dir x c Vx Eq_oof.
-      unfold characterSetMatcher in Eq_oof. focus § _ [] _ § auto destruct in Eq_oof.
-      - search.
-        + Zhelper. MatchState.solve_with lia.
-        + apply Progress.step. lia.
-(*       - injection Eq_oof as ->.
-        unfold CharSet.exist in AutoDest_2. apply List.Exists.failure_kind in AutoDest_2 as [ i [ v [ ? ? ]]].
-        rewrite_canonicalize. discriminate.
-      - injection Eq_oof as ->. rewrite_canonicalize. discriminate. *)
-      - injection Eq_oof as ->.
-        pose proof (@List.Indexing.Int.failure_kind Character) as Falsum. specialize Falsum  with (1 := AutoDest_0).
-        cbn in *. congruence.
-    Qed.
-
-    Lemma positiveLookaroundMatcher: forall m rer dir dir',
-      IntermediateValue.HonoresContinuation m dir' rer ->
-      TerminatingMatcher m dir' rer ->
-      TerminatingMatcher (Definitions.PositiveLookaround.matcher m) dir rer.
-    Proof.
-      intros m rer dir dir' HC_m S_m. intros x c V_x Eq_oof.
-      unfold Definitions.PositiveLookaround.matcher in *.
-      focus § _ [] _ § auto destruct in Eq_oof.
-      + specialize (HC_m _ _ _ V_x AutoDest_) as [ y0 [ V_y0 [ P_x_y0 [=<-] ]]].
-        search.
-      + injection Eq_oof as ->.
-        specialize (S_m _ _ V_x AutoDest_) as [ y0 [ V_y0 [ P_x_y0 Eq_y0 ]]].
-        discriminate.
-    Qed.
-
-    Lemma negativeLookaroundMatcher: forall m rer dir dir',
-      TerminatingMatcher m dir' rer ->
-      TerminatingMatcher (Definitions.NegativeLookaround.matcher m) dir rer.
-    Proof.
-      intros m rer dir dir' S_m. intros x c V_x Eq_oof.
-      unfold Definitions.NegativeLookaround.matcher in *.
-      focus § _ [] _ § auto destruct in Eq_oof.
-      + search.
-      + injection Eq_oof as ->.
-        specialize (S_m _ _ V_x AutoDest_) as [ y0 [ V_y0 [ P_x_y0 Eq_y0 ]]].
-        discriminate.
-    Qed.
-
-    Lemma backreferenceMatcher: forall rer n dir,
-      TerminatingMatcher (backreferenceMatcher rer n dir) dir rer.
-    Proof.
-      unfold TerminatingMatcher. intros rer n dir x c Vx Eq_oof.
-      unfold backreferenceMatcher in Eq_oof. focus § _ [] _ § auto destruct in Eq_oof.
-      - search.
-      - search.
-        + destruct dir; cbn in *; MatchState.solve_with ltac:(cbn in *; lia).
-        + apply Progress.step. MatchState.normalize. cbn in *. lia.
-      - injection Eq_oof as ->.
-        apply List.Exists.failure_kind in AutoDest_3.
-        destruct AutoDest_3 as [ i [ j [ Eq_indexed Eq_oof ]]].
-        focus § _ [] _ § auto destruct in Eq_oof; injection Eq_oof as ->.
-(*         + rewrite_canonicalize. discriminate. *)
-        + pose proof (@List.Indexing.Int.failure_kind Character) as Falsum. specialize Falsum  with (1 := AutoDest_4).
-          cbn in *. congruence.
-(*         + rewrite_canonicalize. discriminate. *)
-        + pose proof (@List.Indexing.Int.failure_kind Character) as Falsum. specialize Falsum  with (1 := AutoDest_3).
-          cbn in *. congruence.
-      - injection Eq_oof as ->.
-        pose proof @List.Indexing.Nat.failure_kind as Falsum.
-        cbn in AutoDest_. focus § _ [] _ § auto destruct in AutoDest_.
-        specialize Falsum  with (1 := AutoDest_).
-        cbn in *. congruence.
-    Qed.
-
-    Lemma compileSubPattern: forall r ctx rer dir m,
-      compileSubPattern r ctx rer dir = Success m ->
-      TerminatingMatcher m dir rer.
-    Proof.
-      induction r; intros ctx rer dir m Eq_m; cbn -[Semantics.repeatMatcher] in Eq_m;
-      focus § _ [] _ § auto destruct.
-      - focus § _ [] _ § auto destruct in Eq_m; injection Eq_m as <-.
-        intros x c Vx H. search.
-      - focus § _ [] _ § auto destruct in Eq_m; injection Eq_m as <-.
-        apply characterSetMatcher.
-      - focus § _ [] _ § auto destruct in Eq_m; injection Eq_m as <-.
-        apply characterSetMatcher.
-      - destruct ae.
-        + focus § _ [] _ § auto destruct in Eq_m; injection Eq_m as <-.
-          apply backreferenceMatcher.
-        + destruct esc; focus § _ [] _ § auto destruct in Eq_m; injection Eq_m as <-; apply characterSetMatcher.
-        + destruct esc; focus § _ [] _ § auto destruct in Eq_m; injection Eq_m as <-; apply characterSetMatcher.
-        + focus § _ [] _ § auto destruct in Eq_m; injection Eq_m as <-.
-          apply backreferenceMatcher.
-      - focus § _ [] _ § auto destruct in Eq_m; injection Eq_m as <-.
-        apply characterSetMatcher.
-      - intros x c Vx H. unfold TerminatingMatcher in IHr1,IHr2.
-        focus § _ [] _ § auto destruct in Eq_m; injection Eq_m as <-.
-        focus § _ [] _ § auto destruct in H.
-        + specialize IHr2 with (1 := AutoDest_0) (2 := Vx) (3 := H) as [ y0 [ Vy0 [ P_x_y0 Eq_oof0 ]]]. search.
-        + injection H as ->. specialize IHr1 with (1 := AutoDest_) (2 := Vx) (3 := AutoDest_1) as [ y0 [ Vy0 [ P_x_y0 Eq_oof0 ]]]. search.
-      - focus § _ [] _ § auto destruct in Eq_m; injection Eq_m as <-.
-        apply repeatMatcher. apply IHr with (1 := AutoDest_).
-      - intros x c Vx H. unfold TerminatingMatcher in IHr1,IHr2.
-        focus § _ [] _ § auto destruct in Eq_m; injection Eq_m as <-.
-        + specialize IHr1 with (1 := AutoDest_) (2 := Vx) (3 := H) as [ y0 [ Vy0 [ P_x_y0 Eq_oof0 ]]].
-          specialize IHr2 with (1 := AutoDest_0) (2 := (MatchState.self_input _ _ _ Vy0)) (3 := Eq_oof0) as [ y1 [ Vy1 [ P_x_y1 Eq_oof1 ]]].
-          search.
-        + specialize IHr2 with (1 := AutoDest_0) (2 := Vx) (3 := H) as [ y0 [ Vy0 [ P_x_y0 Eq_oof0 ]]].
-          specialize IHr1 with (1 := AutoDest_) (2 := (MatchState.self_input _ _ _ Vy0)) (3 := Eq_oof0) as [ y1 [ Vy1 [ P_x_y1 Eq_oof1 ]]].
-          search.
-      - intros x c Vx H. unfold TerminatingMatcher in IHr.
-        focus § _ [] _ § auto destruct in Eq_m; injection Eq_m as <-.
-        specialize IHr with (1 := AutoDest_) (2 := Vx) (3 := H) as [ y [ Vy [ P_x_y Eq_oof ]]].
-        focus § _ [] _ § auto destruct in Eq_oof.
-        + search.
-          focus § _ [] _ § auto destruct in AutoDest_1.
-          MatchState.normalize; try MatchState.solve.
-          apply List.Update.Nat.One.prop_preservation with (3 := AutoDest_1); try assumption.
-          focus § _ [] _ § auto destruct in AutoDest_0; injection AutoDest_0 as <-; constructor; solve [ assumption | lia ].
-        + focus § _ [] _ § auto destruct in AutoDest_1.
-          * spec_reflector Nat.eqb_spec. lia.
-          * rewrite -> List.Update.Nat.One.failure_kind with (f := f) in AutoDest_1 by assumption.
-            injection AutoDest_1 as <-. discriminate.
-        + focus § _ [] _ § auto destruct in AutoDest_0.
-          * injection AutoDest_0 as <-. discriminate.
-          * injection AutoDest_0 as <-. discriminate.
-      - clear_result. subst. intros x c Vx H.
-        focus § _ [] _ § auto destruct in H; try search.
-        focus § _ [] _ § auto destruct in AutoDest_. clear_result. subst.
-        + match goal with | [ H: List.Indexing.Int.indexing _ _ = Failure _ |- _ ] => apply List.Indexing.Int.failure_bounds in H (*; MatchState.solve_with lia*) end.
-          MatchState.solve_with lia.
-        + destruct (RegExp.multiline rer); discriminate.
-      - clear_result. subst. intros x c Vx H.
-        focus § _ [] _ § auto destruct in H; [search| ].
-        focus § _ [] _ § auto destruct in AutoDest_. clear_result. subst.
-        + match goal with | [ H: List.Indexing.Int.indexing _ _ = Failure _ |- _ ] => apply List.Indexing.Int.failure_bounds in H (*; MatchState.solve_with lia*) end.
-          MatchState.solve_with lia.
-        + destruct (RegExp.multiline rer); discriminate.
-      - clear_result. subst. intros x c Vx H.
-        focus § _ [] _ § auto destruct in H; try search.
-        all: lazymatch goal with | [ H: isWordChar _ _ _ = Failure _ |- _ ] =>  unfold isWordChar in H; focus § _ [] _ § auto destruct in H; clear_result; subst end.
-        all: try lazymatch goal with
-            | [ H: wordCharacters _ = Failure _ |- _ ] => exfalso; apply (Compile.wordCharacters _ _ H)
-            | [ H: _ [_] = Failure _ |- _ ] => apply List.Indexing.Int.failure_bounds in H; MatchState.solve_with lia
-            end.
-      - clear_result. subst. intros x c Vx H.
-        focus § _ [] _ § auto destruct in H; try search.
-        all: lazymatch goal with | [ H: isWordChar _ _ _ = Failure _ |- _ ] =>  unfold isWordChar in H; focus § _ [] _ § auto destruct in H; clear_result; subst end.
-        all: try lazymatch goal with
-            | [ H: wordCharacters _ = Failure _ |- _ ] => exfalso; apply (Compile.wordCharacters _ _ H)
-            | [ H: _ [_] = Failure _ |- _ ] => apply List.Indexing.Int.failure_bounds in H; MatchState.solve_with lia
-            end.
-      - focus § _ [] _ § auto destruct in Eq_m; injection Eq_m as <-.
-        apply positiveLookaroundMatcher with (dir' := forward).
-        + apply IntermediateValue.compileSubPattern with (1 := AutoDest_).
-        + apply IHr with (1 := AutoDest_).
-      - focus § _ [] _ § auto destruct in Eq_m; injection Eq_m as <-.
-        apply negativeLookaroundMatcher with (dir' := forward). apply IHr with (1 := AutoDest_).
-      - focus § _ [] _ § auto destruct in Eq_m; injection Eq_m as <-.
-        apply positiveLookaroundMatcher with (dir' := backward).
-        + apply IntermediateValue.compileSubPattern with (1 := AutoDest_).
-        + apply IHr with (1 := AutoDest_).
-      - focus § _ [] _ § auto destruct in Eq_m; injection Eq_m as <-.
-        apply negativeLookaroundMatcher with (dir' := backward). apply IHr with (1 := AutoDest_).
-    Qed.
-
-    Lemma compilePattern: forall r rer input i m,
-      compilePattern r rer = Success m ->
-      m input i <> out_of_fuel.
-    Proof.
-      intros r rer input i m Eq_m. unfold compilePattern in Eq_m.
-      focus § _ [] _ § auto destruct in Eq_m. injection Eq_m as <-.
-      focus § _ (_ [] _) § auto destruct. boolean_simplifier. spec_reflector Nat.leb_spec0.
-      remember (match_state input i (List.repeat None (RegExp.capturingGroupsCount rer))) as x eqn:Eq_x.
-      pose proof (compileSubPattern _ _ _ forward _ AutoDest_ x (fun y => y)) as Falsum.
-      assert (MatchState.Valid (MatchState.input x) rer x) as V_x. {
-        subst x. apply MatchState.valid_init. lia.
-      }
-      focus § _ (_ [] _) § do (fun t => destruct t as [ | f ]; try easy; destruct f; try easy).
-      fforward Falsum. destruct Falsum as [ ? [ _ [ _ ? ]]].
-      subst. discriminate.
-    Qed.
-
-  End main. End Termination.
-
-  Section MatcherInvariant.
-    Context `{CharacterInstance}.
 
     (* For all matcher m *)
     Definition matcher_invariant (m: Matcher) (dir: Direction) (rer: RegExp) :=
@@ -1086,20 +344,626 @@ Module Correctness.
           (* m did some work, yielding a new state y, which was passed to the continuation *)
           (exists y, MatchState.Valid (MatchState.input x) rer y /\ progress dir x (Success (Some y)) /\ c y = m x c).
 
-    Theorem compiledSubPattern_matcher_invariant: forall root r ctx rer dir m,
-        countLeftCapturingParensWithin root nil = RegExp.capturingGroupsCount rer ->
-        Root root r ctx ->
-        EarlyErrors.Pass_Regex root nil ->
-        compileSubPattern r ctx rer dir = Success m ->
-        matcher_invariant m dir rer.
+    Definition fuelBound (min: non_neg_integer) (x: MatchState) (dir: Direction) := min + (MatchState.remainingChars x dir)  + 1.
+
+    Lemma repeatMatcherFuel_satisfies_bound: forall min x rer dir, MatchState.Valid (MatchState.input x) rer x -> fuelBound min x dir <= repeatMatcherFuel min x.
+    Proof. intros. unfold fuelBound,repeatMatcherFuel in *. destruct H as [ ? [ [ Bounds_Ei_x_low Bounds_Ei_x_high ] VC_x ] ]. destruct dir; cbn; lia. Qed.
+
+    Lemma fuelDecreases_min: forall dir min min' x x' b,
+      min' < min -> progress dir x (Success (Some x')) -> fuelBound min x dir <= S b -> fuelBound min' x' dir <= b.
     Proof.
-      intros root r ctx rer dir m.
-      intros Eq_rer R_r P_root Eq_m x c V_x.
-      destruct (m x c) as [ [ | ] | [ | ] ] eqn:Eq_match.
-      - right. apply (IntermediateValue.compileSubPattern _ _ _ _ _ Eq_m _ _ _ V_x Eq_match).
-      - left. reflexivity.
-      - right. apply (Termination.compileSubPattern _ _ _ _ _ Eq_m _ _ V_x Eq_match).
-      - right. apply (Safety.compileSubPattern _ _ _ _ _ _ Eq_rer R_r P_root Eq_m _ _ V_x Eq_match).
+      intros. unfold fuelBound,MatchState.remainingChars in *. inversion H0; destruct dir; inversion H6; subst.
+      - rewrite -> H3 in *. lia.
+      - lia.
     Qed.
-  End MatcherInvariant.
+
+    Lemma fuelDecreases_progress: forall dir rer min x x' b,
+      progress dir x (Success (Some x')) ->
+      ((MatchState.endIndex x) =? (MatchState.endIndex x'))%Z = false ->
+      MatchState.Valid (MatchState.input x) rer x ->
+      MatchState.Valid (MatchState.input x) rer x' ->
+      fuelBound min x dir <= S b ->
+      fuelBound min x' dir <= b.
+    Proof.
+      intros dir rer min x x' b P_x_x' Neq_Eis [ ? [ [ Bei_x_l Bei_x_h ] VC_x ] ] [ ? [ [ B_Ei_x'_l B_Ei_x'_h ] VC_x' ] ] Ineq_fuel.
+      dependent destruction P_x_x'. rename H into Eq_inp_x_x', H0 into Dp_x_x'.
+      unfold fuelBound, MatchState.remainingChars in *.
+      rewrite <- Eq_inp_x_x' in *.
+      spec_reflector Z.eqb_spec.
+      dependent destruction Dp_x_x'; lia.
+    Qed.
+
+    Ltac base_reasoning := autounfold with result_wrappers in *; Result.inject_all; subst; repeat lazymatch goal with
+    | [ |- ?x = ?x \/ _ ] => left; reflexivity
+    | [ |- Failure _ = Success None \/ _ ] => right
+    end.
+
+    Ltac search := base_reasoning; lazymatch goal with
+    | [ H: ?c ?y = ?r |- _ \/ (exists x, MatchState.Valid _ _ x /\ progress ?dir _ _ /\ ?c x = ?r) ] => right; search
+    | [ |- _ \/ (exists x, MatchState.Valid _ _ x /\ progress ?dir _ _ /\ ?c x = ?c ?y) ] => right; search
+    | [ H: ?P |- _ \/ ?P ] => right; apply H
+    | [ H: ?c ?y = ?r |- exists x, MatchState.Valid _ _ x /\ progress ?dir _ _ /\ ?c x = ?r ] =>
+      exists y; split; [ | split ];
+      [ try Progress.solve
+      | try solve [Progress.saturate]
+      | apply H ]
+    | [ |- exists x, MatchState.Valid _ _ x /\ progress ?dir _ _ /\ ?c x = ?c ?y ] =>
+      exists y; split; [ | split ];
+      [ try Progress.solve
+      | try solve [Progress.saturate]
+      | reflexivity ]
+    end.
+
+    Ltac eval_matcher H := lazymatch goal with
+    | [ |- matcher_invariant ?m _ _ ] =>
+        let x := fresh "x" in
+        let c := fresh "c" in
+        let Vx := fresh "V_" x in
+        intros x c Vx; destruct m eqn:H; cbn in H; focus § _ [] _ § auto destruct in H
+    | [ H: ?m ?x ?c = ?res |- ?res = _ \/ (exists y : MatchState, MatchState.Valid (MatchState.input ?x) _ y /\ progress _ ?x (Success (Some y)) /\ ?c y = ?res)] =>
+        cbn in H; focus § _ [] _ § auto destruct in H
+    end; autounfold with result_wrappers in *; repeat match goal with [ H: Success _ = Success _ |- _ ] => injection H as H end.
+    Tactic Notation "run" "matcher" "as" ident(H) := eval_matcher H.
+
+    Ltac quick_math := repeat (
+      boolean_simplifier ||
+      spec_reflector Nat.eqb_spec ||
+      spec_reflector Nat.leb_spec0 ||
+      spec_reflector Z.eqb_spec ||
+      spec_reflector Z.ltb_spec0 ||
+      spec_reflector Z.leb_spec0 ||
+      normalize_Z_comp).
+
+    Lemma characterSetMatcher: forall rer A invert dir,
+      matcher_invariant (characterSetMatcher rer A invert dir) dir rer.
+    Proof.
+      intros rer A invert dir. unfold characterSetMatcher.
+      run matcher as Matching; autounfold with result_wrappers in *.
+      1-3: search.
+      - search. +  Zhelper. MatchState.solve_with lia. + apply Progress.step. lia.
+      - search. +  Zhelper. MatchState.solve_with lia. + apply Progress.step. lia.
+      - base_reasoning. 
+        apply List.Indexing.Int.failure_bounds in AutoDest_0.
+        quick_math.
+        destruct V_x as [ Eq_str [ [ ? ? ] _ ]].
+        destruct dir; cbn in *.
+        + replace (Z.min (MatchState.endIndex x) (MatchState.endIndex x + 1)) with (MatchState.endIndex x) in * by lia. lia.
+        + replace (Z.min (MatchState.endIndex x) (MatchState.endIndex x - 1)) with (MatchState.endIndex x - 1)%Z in * by lia. lia.
+    Qed.
+
+    Lemma mi_application_match: forall (m: Matcher) dir rer x c z
+      (MI: matcher_invariant m dir rer)
+      (V_x: MatchState.Valid (MatchState.input x) rer x)
+      (Eq_z: m x c = Success (Some z)),
+      exists y, MatchState.Valid (MatchState.input x) rer y /\ progress dir x (Success (Some y)) /\ c y = (Success (Some z)).
+    Proof. intros. specialize (MI x c V_x) as [H | H]. - rewrite -> Eq_z in H. discriminate. - rewrite -> Eq_z in H. apply H. Qed.
+
+    Lemma mi_application_success: forall (m: Matcher) dir rer x c z
+      (MI: matcher_invariant m dir rer)
+      (V_x: MatchState.Valid (MatchState.input x) rer x)
+      (Eq_z: m x c = Success z),
+      z = None \/ exists y, MatchState.Valid (MatchState.input x) rer y /\ progress dir x (Success (Some y)) /\ c y = (Success z).
+    Proof. intros. specialize (MI x c V_x) as [H | H]. - rewrite -> Eq_z in H. injection H as ->. left. reflexivity. - rewrite -> Eq_z in H. right. apply H. Qed.
+
+    Lemma mi_application_failure: forall (m: Matcher) dir rer x c f
+      (MI: matcher_invariant m dir rer)
+      (V_x: MatchState.Valid (MatchState.input x) rer x)
+      (Eq_z: m x c = Failure f),
+      exists y, MatchState.Valid (MatchState.input x) rer y /\ progress dir x (Success (Some y)) /\ c y = Failure f.
+    Proof. intros. specialize (MI x c V_x) as [H | H]. - rewrite -> Eq_z in H. discriminate. - rewrite -> Eq_z in H. apply H. Qed.
+
+
+    Lemma mi_application_generic: forall (m: Matcher) dir rer x c r
+      (MI: matcher_invariant m dir rer)
+      (V_x: MatchState.Valid (MatchState.input x) rer x)
+      (Eq_z: m x c = r),
+      r = None \/ exists y, MatchState.Valid (MatchState.input x) rer y /\ progress dir x (Success (Some y)) /\ c y = r.
+    Proof. intros. specialize (MI x c V_x) as [? | ?]; subst. - left; assumption. - right; assumption. Qed.
+
+    Ltac apply_mi_in_goal H By :=
+      lazymatch type of H with
+      | matcher_invariant ?m ?dir ?rer =>
+        lazymatch goal with
+        | [|- m ?x ?c = Success None \/ (exists y, _ /\ _ /\ _ y = m ?x ?c) ] =>
+            let tmp := fresh "Tmp" in
+            pose proof (H x c) as [-> | tmp]; [ By | left; reflexivity |
+              let y := fresh "x" in
+              let Vy := fresh "V_" y in
+              let Py := fresh "P_" y in
+              destruct tmp as (y & Vy & Py & <-) ]
+        | [|- _ ] => fail "Goal does not look like a matcher invariant..."
+        end
+      | ?T => fail "Applied invariant has incorrect type:" T
+      end.
+
+    Ltac einstance H := lazymatch type of H with
+    | forall (_: ?T), _ =>
+        let x := fresh "eTmp" in
+        evar (x : T);
+        let x' := (eval unfold x in x) in
+        clear x; specialize (H x'); einstance H
+    | _ => idtac
+    end.
+
+    Ltac apply_mi_in_hyp H In As By :=
+      let apply_theorems := fun H m dir rer =>
+        lazymatch type of In with
+        | ?m' ?x ?c = ?r =>
+            unify m m';
+            lazymatch r with
+            | Success (Some ?y) => apply (mi_application_match m dir rer x c y H) in In as As; [ | .. | By ]
+            | Success ?y        => apply (mi_application_success m dir rer x c y H) in In as As; [ | .. | By ]
+            | Failure ?f        => apply (mi_application_failure m dir rer x c f H) in In as As; [ | .. | By ]
+            | ?r                => apply (mi_application_generic m dir rer x c r H) in In as As; [ | .. | By ]
+            | ?T => fail "Target hypothesis has incorrect type:" T
+            end
+        | ?T => fail "Target hypothesis has incorrect type (or could not unify):" T
+        end
+      in
+      let check_trimmed := fun H => 
+        lazymatch type of H with
+        | matcher_invariant ?m ?dir ?rer => apply_theorems H m dir rer
+        | ?T => fail "Applied invariant has incorrect type:" T
+        end
+      in
+      lazymatch type of H with
+      | forall _, _ =>
+          let tmp := fresh "Tmp" in
+          pose proof H as tmp;
+          einstance tmp;
+          check_trimmed tmp;
+          clear tmp
+      | _ => check_trimmed H
+      end.
+
+    Tactic Notation "apply_mi" constr(H) := (apply_mi_in_goal H idtac).
+    Tactic Notation "apply_mi" constr(H) "by" tactic1(By) := (apply_mi_in_goal H By).
+    Tactic Notation "apply_mi" constr(H) "in" hyp(In) "as" simple_intropattern(As) := (apply_mi_in_hyp H In As idtac).
+    Tactic Notation "apply_mi" constr(H) "in" hyp(In) "as" simple_intropattern(As) "by" tactic1(By) := (apply_mi_in_hyp H In As By).
+
+    Ltac repeatMatcher_as_matcher := lazymatch goal with
+    | [ _: context[ repeatMatcher' ?m ?min ?max ?greedy ?x ?c ?parenIndex ?parenCount ?fuel ] |- _ ] =>
+        replace (repeatMatcher' m min max greedy x c parenIndex parenCount fuel) with (Definitions.RepeatMatcher.matcher m min max greedy parenIndex parenCount fuel x c) in * by reflexivity
+    end.
+
+    Lemma repeatMatcher': forall greedy parenIndex parenCount m rer dir,
+      Captures.Valid rer parenIndex parenCount ->
+      matcher_invariant m dir rer ->
+      forall fuel min x,
+        fuelBound min x dir <= fuel ->
+      forall max c res,
+        Definitions.RepeatMatcher.matcher m min max greedy parenIndex parenCount fuel x c = res ->
+        (* such that x is valid *)
+        MatchState.Valid (MatchState.input x) rer x ->
+        (* Then either *)
+          (* The match fails *)
+          (res = failure) \/
+          (* or *)
+          (* m did some work, yielding a new state y, which was passed to the continuation *)
+          (exists y, MatchState.Valid (MatchState.input x) rer y /\ progress dir x (Success (Some y)) /\ c y = res).
+    Proof.
+      intros greedy parenIndex parenCount m rer dir V_captures MI_m. induction fuel.
+      - intros min x Ineq_fuel. exfalso. unfold fuelBound,MatchState.remainingChars in Ineq_fuel. lia.
+      - intros min x Ineq_fuel max c res Eq_res V_x.
+        run matcher as Matching; try search.
+        + apply_mi MI_m in Eq_res as [ ? | (y0 & ? & ? & Matching) ] by MatchState.solve; [ search | ].
+          repeatMatcher_as_matcher.
+          focus § _ [] _ § auto destruct in Matching; [ search | ].
+          specialize IHfuel with (2 := Matching). fforward IHfuel by try MatchState.solve.
+          1: {
+            apply fuelDecreases_min with (x := x) (min := min); [ | Progress.solve | assumption ].
+            quick_math. lia.
+          }
+          destruct IHfuel as [ ? | (y1 & V_y1 & P_y0_y1 & Eq_res) ]; [ search | right ].
+          search.
+        + apply_mi MI_m in Eq_res as [ ? | (y0 & ? & ? & Matching) ] by MatchState.solve; [ search | ].
+          repeatMatcher_as_matcher.
+          focus § _ [] _ § auto destruct in Matching; [ search | ].
+          specialize IHfuel with (2 := Matching). fforward IHfuel by try MatchState.solve.
+          1: {
+            quick_math; subst.
+            apply fuelDecreases_progress with (x := x) (rer := rer) ; [ Progress.solve | quick_math; congruence | MatchState.solve | MatchState.solve | assumption ].
+          }
+          destruct IHfuel as [ ? | (y1 & V_y1 & P_y0_y1 & Eq_res) ]; [ search | right ].
+          search.
+        + apply_mi MI_m in AutoDest_3 as [ ? | (y0 & ? & ? & Matching) ] by MatchState.solve; [ search | ].
+          repeatMatcher_as_matcher.
+          focus § _ [] _ § auto destruct in Matching; [ search | ].
+          specialize IHfuel with (2 := Matching). fforward IHfuel by try MatchState.solve.
+          1: {
+            quick_math; subst.
+            apply fuelDecreases_progress with (x := x) (rer := rer) ; [ Progress.solve | quick_math; congruence | MatchState.solve | MatchState.solve | assumption ].
+          }
+          destruct IHfuel as [ ? | (y1 & V_y1 & P_y0_y1 & ?) ]; [ search | right ].
+          search.
+        + apply_mi MI_m in AutoDest_3 as (y0 & V_y0 & P_x_y0 & Matching) by MatchState.solve.
+          repeatMatcher_as_matcher.
+          focus § _ [] _ § auto destruct in Matching.
+          specialize IHfuel with (2 := Matching). fforward IHfuel by try MatchState.solve.
+          1: {
+            quick_math; subst.
+            apply fuelDecreases_progress with (x := x) (rer := rer) ; [ Progress.solve | quick_math; congruence | MatchState.solve | MatchState.solve | assumption ].
+          }
+          destruct IHfuel as [ ? | (y1 & V_y1 & P_y0_y1 & ?) ]; [ search | right ].
+          search.
+        + Search Captures.Valid. unfold Captures.Valid in V_captures.
+          apply List.Update.Nat.Batch.failure_bounds in AutoDest_0. (* TODO: use pinpoint *)
+          destruct V_x as [ _ [ _ [ VCL_x _ ]]]. rewrite -> VCL_x in *. repeat rewrite Nat.add_sub in *. contradiction.
+    Qed.
+
+    Lemma repeatMatcher: forall m min max greedy parenIndex parenCount dir rer,
+      Captures.Valid rer parenIndex parenCount ->
+      matcher_invariant m dir rer ->
+      matcher_invariant (fun x c => repeatMatcher m min max greedy x c parenIndex parenCount) dir rer.
+    Proof.
+      intros m min max greedy parenIndex parenCount dir rer V_captures MI_m x c V_x.
+      apply (repeatMatcher' _ _ _ _ _ _ V_captures MI_m (repeatMatcherFuel min x) _ x ltac:(eauto using repeatMatcherFuel_satisfies_bound) _ _ _ ltac:(apply eq_refl) V_x).
+    Qed.
+
+    Lemma positiveLookaroundMatcher: forall m rer dir dir',
+      matcher_invariant m dir' rer ->
+      matcher_invariant (Definitions.PositiveLookaround.matcher m) dir rer.
+    Proof.
+      intros m rer dir dir' MI_m. unfold Definitions.PositiveLookaround.matcher.
+      run matcher as Matching; autounfold with result_wrappers in *;
+        match goal with | [ H: m _ _ = _ _ |- _ ] => rename H into Eq_m end.
+      - search.
+      - apply_mi MI_m in Eq_m as (? & ? & _ & [=->]) by assumption. search.
+      - apply_mi MI_m in Eq_m as (? & ? & _ & [=->]) by assumption. search.
+      - apply_mi MI_m in Eq_m as (? & _ & _ & ?) by assumption. discriminate.
+    Qed.
+
+    Lemma negativeLookaroundMatcher: forall m rer dir dir',
+      matcher_invariant m dir' rer ->
+      matcher_invariant (Definitions.NegativeLookaround.matcher m) dir rer.
+    Proof.
+      intros m rer dir dir' MI_m. unfold Definitions.NegativeLookaround.matcher.
+      run matcher as Matching; autounfold with result_wrappers in *.
+      - search.
+      - search.
+      - search.
+      - match goal with | [ H: m _ _ = _ _ |- _ ] => rename H into Eq_m end.
+        apply_mi MI_m in Eq_m as (? & _ & _ & ?) by assumption. discriminate.
+    Qed.
+
+    Lemma captured_range_diff: forall str rer x i r,
+      MatchState.Valid str rer x ->
+      List.Indexing.Nat.indexing (MatchState.captures x) i = Success (Some r) ->
+      (0 <= (CaptureRange.endIndex r) - (CaptureRange.startIndex r))%Z.
+    Proof. intros. MatchState.normalize. specialize (VCF_captures_x _ _ H0). dependent destruction VCF_captures_x. lia. Qed.
+
+    Lemma directional_min_rewrite: forall i r dir,
+      (0 <= r)%Z ->
+      Z.min
+        (i)
+        (if dir == forward
+           then (i + r)%Z
+           else (i - r)%Z)
+      = if dir == forward then i else (i - r)%Z.
+    Proof.
+      intros ? ? [ | ] ?; cbn;
+        lazymatch goal with
+          | [ |- context[ Z.min ?i (?i + ?r)%Z ] ] =>
+              replace (Z.min i (i + r)) with i in * by lia
+          | [ |- context[ Z.min ?i (?i - ?r)%Z ] ] =>
+              replace (Z.min i (i - r)) with (i - r)%Z in * by lia
+          end; reflexivity.
+    Qed.
+
+    Lemma backreferenceMatcher: forall rer n dir,
+      (positive_to_non_neg n) <= RegExp.capturingGroupsCount rer ->
+      matcher_invariant (backreferenceMatcher rer n dir) dir rer.
+    Proof.
+      intros rer n dir Eq_rer. unfold backreferenceMatcher.
+      run matcher as Matching; autounfold with result_wrappers in *.
+      - search.
+      - search.
+      - search.
+      - search.
+        + destruct dir; cbn in *; MatchState.solve_with ltac:(cbn in *; lia).
+        + apply Progress.step. eapply captured_range_diff; eassumption.
+      - search.
+      - search.
+        + destruct dir; cbn in *; MatchState.solve_with ltac:(cbn in *; lia).
+        + apply Progress.step. eapply captured_range_diff; eassumption.
+      - (* An out-of-bound happend while indexing the input string: we prove it is actually impossible. *)
+        injection Matching as ->.
+
+        (* The maximal offset (r = endIndex - startIndex) is positive *)
+        remember (CaptureRange.endIndex t - CaptureRange.startIndex t)%Z as r.
+        assert (0 <= r)%Z as Pos_r. { subst r. eapply captured_range_diff; eassumption. }
+
+        (* The end and start of the range and the current index, are in bounds *)
+        destruct V_x as (_ & ? & _ & V_range).
+        match goal with
+        | [ H: List.Indexing.Nat.indexing (MatchState.captures x) _ = Success (Some _) |- _ ] =>
+            specialize (V_range _ _ H); dependent destruction V_range
+        end.
+        unfold IteratorOn in *.
+
+        (* Get rid of Z.min *)
+        rewrite -> directional_min_rewrite  in * by assumption.
+
+        (* There must be an offset i (0 <= i < r) where the indexing fails *)
+        match goal with | [ H: List.Exists.exist _ _ = Failure _ |- _ ] => rename H into Indexing_failure end.
+        apply List.Exists.failure_kind in Indexing_failure.
+        destruct Indexing_failure as [ i [ j [ Eq_indexed Indexing_failure ]]].
+        pose proof (List.Range.Int.Bounds.indexing _ _ _ _ Eq_indexed) as ->. apply List.Indexing.Int.success_bounds in Eq_indexed.
+        rewrite -> List.Range.Int.Bounds.length in *. cbn in *.
+
+        (* Conclude by case analysis *)
+        focus § _ [] _ § auto destruct in Indexing_failure; injection Indexing_failure as ->;
+          match goal with
+          | [ H: List.Indexing.Int.indexing _ _ = Failure _ |- _ ] =>
+              apply List.Indexing.Int.failure_bounds in H as [Indexing_failure | Indexing_failure]
+          end; destruct dir.
+        all: cbn in *; lia.
+      - (* The capture group does not exist; we prove it is actually impossible. *)
+        injection Matching as ->.
+        match goal with | [ H: List.Indexing.Nat.indexing _ _ = Failure _ |- _ ] => rename H into Eq_failure end.
+        apply List.Indexing.Nat.failure_bounds in Eq_failure.
+        destruct V_x as (_ & _ & ? & _). pose proof (NonNegInt.pos n). lia.
+    Qed.
+
+    Inductive Guard := guard.
+    Ltac node_induction :=
+      lazymatch goal with
+      | [|- forall r ctx, Root ?root (r, ctx) -> @?P r ctx ] =>
+          let P' := (eval cbn in (fun p => forall _: Guard, P (fst p) (snd p))) in
+          let Tmp1 := fresh "r" in let Tmp2 := fresh "ctx" in let Tmp3 := fresh "Tmp" in 
+          intros Tmp1 Tmp2 Tmp3; generalize guard; generalize dependent Tmp3; generalize dependent Tmp2; generalize dependent Tmp1;
+          apply (Node_ind root P')
+      end;
+      repeat lazymatch goal with
+      | [ H: Guard -> _ |- _ ] => specialize (H guard)
+      | [|- forall a: Guard, _ ] => fail
+      | [|- forall (_: ?T), _ ] => match type of T with
+        | Prop => let H := fresh "IH" in intros H
+        | _ => intros ?
+        end
+      end; intros _.
+
+
+    Ltac compileSubPattern_helper := repeat match goal with
+    | [ IH: forall _ _, compileSubPattern ?r _ _ _ = Success _ -> _, H: compileSubPattern ?r _ _ _ = Success _  |- _ ] =>
+        specialize IH with (1 := H)
+    end.
+
+    Lemma isWordChar_failure: forall rer x f, isWordChar rer (MatchState.input x) (MatchState.endIndex x) = Failure f -> ~ MatchState.Valid (MatchState.input x) rer x.
+    Proof. unfold isWordChar. cbn. intros rer x f H Falsum. focus § _ [] _ § auto destruct in H. apply List.Indexing.Int.failure_bounds in AutoDest_0. quick_math. MatchState.solve_with lia. Qed.
+    Lemma isWordChar_failure_min: forall rer x f, isWordChar rer (MatchState.input x) (MatchState.endIndex x - 1)%Z = Failure f -> ~ MatchState.Valid (MatchState.input x) rer x.
+    Proof. unfold isWordChar. cbn. intros rer x f H Falsum. focus § _ [] _ § auto destruct in H. apply List.Indexing.Int.failure_bounds in AutoDest_0. quick_math. MatchState.solve_with lia. Qed.
+
+    Ltac pinpoint_failure := repeat match goal with
+      | [ H: _ = Failure _ |- _ ] => progress (focus § _ [] _ § auto destruct in H); injection H as ->
+      | [ H: List.Update.Nat.One.update _ _ _ = Failure _ |- _ ] => apply List.Update.Nat.One.failure_bounds in H
+      | [ H: List.Indexing.Int.indexing _ _ = Failure _ |- _ ] => apply List.Indexing.Int.failure_bounds in H
+      | [ H: isWordChar _ _ _ = Failure _ |- _ ] => apply isWordChar_failure in H + apply isWordChar_failure_min in H
+      end.
+
+    Lemma compileSubPattern: forall root rer,
+      countLeftCapturingParensWithin root nil = RegExp.capturingGroupsCount rer ->
+      EarlyErrors.Pass_Regex root nil ->
+      forall r ctx,
+      Root root (r, ctx) ->
+      forall  dir m,
+      compileSubPattern r ctx rer dir = Success m ->
+      matcher_invariant m dir rer.
+    Proof.
+      intros root rer Eq_rer EE_root.
+      node_induction.
+      all: intros dir m Eq_m; cbn -[Semantics.repeatMatcher] in Eq_m.
+      - (* Empty *)
+        injection Eq_m as <-. intros x c V_x. right. exists x. split_conjs; [ assumption | Progress.solve | reflexivity ].
+      - (* Character *)
+        injection Eq_m as <-. apply characterSetMatcher.
+      - (* Dot *)
+        injection Eq_m as <-. apply characterSetMatcher.
+      - (* AtomEscape *)
+        destruct ae.
+        + (* Numbered backref *)
+          focus § _ [] _ § auto destruct in Eq_m; injection Eq_m as <-.
+          apply backreferenceMatcher. quick_math. assumption.
+        + (* Character class *)
+          destruct esc; focus § _ [] _ § auto destruct in Eq_m; injection Eq_m as <-; apply characterSetMatcher.
+        + (* Character *)
+          destruct esc; focus § _ [] _ § auto destruct in Eq_m; injection Eq_m as <-; apply characterSetMatcher.
+        + (* Named backref *)
+          focus § _ [] _ § auto destruct in Eq_m; injection Eq_m as <-.
+          apply backreferenceMatcher. quick_math. cbn in *.
+          apply List.Unique.success in AutoDest_0. destruct s. cbn in *.
+          assert (List.Indexing.Nat.indexing (groupSpecifiersThatMatch (AtomEsc (GroupEsc id)) ctx id) 0 = Success (r, l)) as Eq_indexed. {
+            match goal with | [ H: _ = (r, l) :: nil |- _ ] => setoid_rewrite -> H end.
+            reflexivity.
+          }
+          pose proof (EarlyErrors.groupSpecifiersThatMatch_is_filter_map (AtomEsc (GroupEsc id)) ctx id) as (f & _ & Def_f).
+          apply Def_f in Eq_indexed. destruct Eq_indexed as (ctx' & ? & Eq_indexed).
+          subst. destruct (countLeftCapturingParensBefore_impl ctx' + 1) eqn:Eq; try lia. cbn in *.
+          apply Zipper.Walk.soundness in Eq_indexed. eapply Zipper.Down.same_root_down in Eq_indexed; [ | eapply IH ]. cbn in *.
+          pose proof (EarlyErrors.countLeftCapturingParensBefore_contextualized _ _ _ Eq_indexed EE_root).
+          subst. unfold countLeftCapturingParensBefore,countLeftCapturingParensWithin in *. cbn in *.
+          apply NonNegInt.to_positive_soundness in AutoDest_1.
+          lia.
+      - (* Character class *)
+        focus § _ [] _ § auto destruct in Eq_m; auto using Compile.compileCharacterClass.
+        injection Eq_m as <-. apply characterSetMatcher.
+      - (* Disjunction *)
+        focus § _ [] _ § auto destruct in Eq_m. injection Eq_m as <-.
+        compileSubPattern_helper.
+        run matcher as Matching; rewrite <- Matching, <- ?AutoDest_1 in *; auto.
+      - (* Quantifier *)
+        focus § _ [] _ § auto destruct in Eq_m. injection Eq_m as <-. apply repeatMatcher.
+        + intros i v Eq_indexed.
+          pose proof (List.Indexing.Nat.success_bounds _ _ _ Eq_indexed). rewrite -> List.Range.Nat.Bounds.length in *.
+          apply List.Range.Nat.Bounds.indexing in Eq_indexed.
+          pose proof (EarlyErrors.countLeftCapturingParensBefore_contextualized _ _ _ IH EE_root).
+          unfold countLeftCapturingParensBefore,countLeftCapturingParensWithin in *. cbn in *. lia.
+        + compileSubPattern_helper. assumption.
+      - (* Sequence *)
+        destruct dir; cbn in *.
+        + focus § _ [] _ § auto destruct in Eq_m. injection Eq_m as <-.
+          compileSubPattern_helper.
+          run matcher as Matching; rewrite <- Matching.
+          * apply_mi IH0 by assumption. apply_mi IH2 by MatchState.solve. right. search. Progress.normalize. lia.
+          * apply_mi IH0 by assumption. apply_mi IH2 by MatchState.solve. right. search. Progress.normalize. lia.
+        + focus § _ [] _ § auto destruct in Eq_m. injection Eq_m as <-.
+          compileSubPattern_helper.
+          run matcher as Matching; rewrite <- Matching.
+          * apply_mi IH2 by assumption. apply_mi IH0 by MatchState.solve. right. search. Progress.normalize. lia.
+          * apply_mi IH2 by assumption. apply_mi IH0 by MatchState.solve. right. search. Progress.normalize. lia.
+      - (* (Capturing) Group *)
+        focus § _ [] _ § auto destruct in Eq_m. injection Eq_m as <-.
+        compileSubPattern_helper.
+        run matcher as Matching.
+        + (* Run succeeded *)
+          apply_mi IH0 in Matching as [? | (y & V_y & P_y & Eq_s)] by assumption.
+          * subst. left. reflexivity.
+          * focus § _ [] _ § auto destruct in Eq_s.
+            focus § _ [] _ § auto destruct in AutoDest_1.
+            search.
+        + (* Failure occured => toward contradiction *)
+          apply_mi IH0 in Matching as (y & V_y & P_y & Eq_f) by assumption.
+          focus § _ [] _ § auto destruct in Eq_f.
+          * (* Cause: call to continuation *)
+            match goal with | [ H: _ = Success ?s |- _ ] => check_type s (list (option CaptureRange)); focus § _ [] _ § auto destruct in H end.
+            search.
+          * (* Cause: capture update *)
+            injection Eq_f as ->.
+            match goal with | [ H: _ = Failure ?f |- _ ] => focus § _ [] _ § auto destruct in H end.
+            -- (* Count left paren is -1 *)
+                quick_math. lia.
+            -- (* Update oob *)
+               pinpoint_failure.
+               pose proof (countLeftCapturingParensBefore_contextualized ctx _ _ ltac:(eassumption) ltac:(eassumption)).
+               destruct V_y as (_ & _ & Tmp & _); rewrite <- Tmp in *. rewrite <- Eq_rer in *. unfold countLeftCapturingParensWithin,countLeftCapturingParensBefore in *. cbn in *.
+               MatchState.solve_with lia.
+          * (* Cause: invalid range *)
+            injection Eq_f as ->.
+            lazymatch goal with | [ H: _ = Failure _ |- _ ] => destruct dir; focus § _ [] _ § auto destruct in H; injection H as <- end. 
+            all: boolean_simplifier; quick_math; Progress.normalize; lia.
+      - (* Match start *)
+        injection Eq_m as <-. run matcher as Matching; try search.
+        injection Matching as ->.
+        pinpoint_failure.
+        MatchState.solve_with lia.
+      - (* Match end *)
+        injection Eq_m as <-. run matcher as Matching; try search.
+        injection Matching as ->.
+        pinpoint_failure.
+        MatchState.solve_with lia.
+      - (* Word boundary *)
+        injection Eq_m as <-. run matcher as Matching; try search; injection Matching as <-; pinpoint_failure; contradiction.
+      - (* Non word boundary *)
+        injection Eq_m as <-. run matcher as Matching; try search; injection Matching as <-; pinpoint_failure; contradiction.
+      - (* Lookahead *)
+        focus § _ [] _ § auto destruct in Eq_m. injection Eq_m as <-. apply positiveLookaroundMatcher with (dir' := forward). auto.
+      - (* Negative lookahead *)
+        focus § _ [] _ § auto destruct in Eq_m. injection Eq_m as <-. apply negativeLookaroundMatcher with (dir' := forward). auto.
+      - (* Lookbehind *)
+        focus § _ [] _ § auto destruct in Eq_m. injection Eq_m as <-. apply positiveLookaroundMatcher with (dir' := backward). auto.
+      - (* Negative lookbehind *)
+        focus § _ [] _ § auto destruct in Eq_m. injection Eq_m as <-. apply negativeLookaroundMatcher with (dir' := backward). auto.
+    Qed.
+  End main. End MatcherInvariant.
+
+  Lemma initialState_validity `{ci: CharacterInstance}: forall input i rer,
+    i <= (length input) ->
+    MatchState.Valid input rer (match_state input (Z.of_nat i) (repeat None (capturingGroupsCount rer))).
+  Proof.
+    constructor.
+    + subst. MatchState.solve.
+    + subst. split_conjs.
+      * subst. cbn. constructor; lia.
+      * cbn. rewrite -> List.repeat_length. reflexivity.
+      * intros j v Indexed.
+        cbn in Indexed. apply List.Indexing.Nat.repeat in Indexed. subst.
+        constructor.
+  Qed.
+
+  Theorem monotony `{ci: CharacterInstance}: forall r rer input i m,
+    EarlyErrors.Pass_Regex r nil ->
+    countLeftCapturingParensWithin r nil = RegExp.capturingGroupsCount rer ->
+    compilePattern r rer = Success m ->
+    progress forward (match_state input (Z.of_nat i) (List.repeat None (RegExp.capturingGroupsCount rer))) (m input i).
+  Proof.
+    intros r rer input i m EE_root Eq_rer Eq_m.
+    unfold compilePattern in *.
+    focus § _ [] _ § auto destruct in Eq_m. injection Eq_m as <-.
+    cbn. focus § _ _ _ [] § auto destruct.
+    - constructor.
+    - boolean_simplifier. spec_reflector Nat.leb_spec0.
+      (* Assert that the start state is valid *)
+      focus § _ _ [] _ § do (fun y => remember y as x eqn:Eq_x).
+      assert (MatchState.Valid (MatchState.input x) rer x) as V_x. {
+        subst. apply initialState_validity. assumption.
+      }
+      (* Use the matcher invariant *)
+      pose proof (MatcherInvariant.compileSubPattern) as H.
+      specialize H with (1 := Eq_rer) (2 := EE_root) (3 := ltac:(apply Zipper.Root.id)) (4 := AutoDest_).
+      specialize (H x (fun y => y) V_x).
+      (* Match either failed or succeeded *)
+      destruct H as [ -> | (y & ? & ? & <-) ].
+      + (* Failure => vacuously true *)
+        constructor.
+      + (* Success => Direct from matcher invariant *)
+        Progress.solve.
+  Qed.
+
+  Theorem termination `{ci: CharacterInstance}: forall r rer input i m,
+    EarlyErrors.Pass_Regex r nil ->
+    countLeftCapturingParensWithin r nil = RegExp.capturingGroupsCount rer ->
+    compilePattern r rer = Success m ->
+    (m input i) <> out_of_fuel.
+  Proof.
+    intros r rer input i m EE_root Eq_rer Eq_m.
+    unfold compilePattern in *.
+    focus § _ [] _ § auto destruct in Eq_m. injection Eq_m as <-.
+    cbn. focus § _ (_ [] _) § auto destruct.
+    boolean_simplifier. spec_reflector Nat.leb_spec0.
+    (* Assert that the start state is valid *)
+    focus § _ (_ (_ [] _) _) § do (fun y => remember y as x eqn:Eq_x).
+    assert (MatchState.Valid (MatchState.input x) rer x) as V_x. {
+      subst. apply initialState_validity. assumption.
+    }
+    (* Use the matcher invariant *)
+    pose proof (MatcherInvariant.compileSubPattern) as H.
+    specialize H with (1 := Eq_rer) (2 := EE_root) (3 := ltac:(apply Zipper.Root.id)) (4 := AutoDest_).
+    specialize (H x (fun y => y) V_x).
+    (* Match either failed or succeeded *)
+    destruct H as [ -> | (y & ? & ? & <-) ].
+    + (* Failure => vacuously true *)
+      easy.
+    + (* Success => contradiction, due to continuation *)
+      easy.
+  Qed.
+
+  Theorem no_failure `{ci: CharacterInstance}: forall r rer input i m,
+    EarlyErrors.Pass_Regex r nil ->
+    countLeftCapturingParensWithin r nil = RegExp.capturingGroupsCount rer ->
+    compilePattern r rer = Success m ->
+    (i < length input) ->
+    (m input i) <> match_assertion_failed.
+  Proof.
+    intros r rer input i m EE_root Eq_rer Eq_m Bound_i.
+    unfold compilePattern in *.
+    focus § _ [] _ § auto destruct in Eq_m. injection Eq_m as <-.
+    cbn. focus § _ (_ [] _) § auto destruct.
+    - boolean_simplifier. spec_reflector Nat.leb_spec0. lia.
+    - boolean_simplifier. spec_reflector Nat.leb_spec0.
+      (* Assert that the start state is valid *)
+      focus § _ (_ (_ [] _) _) § do (fun y => remember y as x eqn:Eq_x).
+      assert (MatchState.Valid (MatchState.input x) rer x) as V_x. {
+        subst. apply initialState_validity. assumption.
+      }
+      (* Use the matcher invariant *)
+      pose proof (MatcherInvariant.compileSubPattern) as H.
+      specialize H with (1 := Eq_rer) (2 := EE_root) (3 := ltac:(apply Zipper.Root.id)) (4 := AutoDest_).
+      specialize (H x (fun y => y) V_x).
+      (* Match either failed or succeeded *)
+      destruct H as [ -> | (y & ? & ? & <-) ].
+      + (* Failure => vacuously true *)
+        easy.
+      + (* Success => contradiction, due to continuation *)
+        easy.
+  Qed.
 End Correctness.
