MECMAR/utils/Typeclasses.v
@@ -20,3 +20,4 @@ Instance eqdec_nat: EqDec nat := { eq_dec := Nat.eq_dec }.
 Instance eqdec_string: EqDec String.string := { eq_dec := String.string_dec }.
 #[refine] Instance eqdec_positive: EqDec positive := {}. decide equality. Defined.
 #[refine] Instance eqdec_option {T: Type} `{EqDec T}: EqDec (option T) := {}. decide equality; apply EqDec.eq_dec. Defined.
+#[refine] Instance eqdec_list {T: Type} `{EqDec T}: EqDec (list T) := {}. decide equality; apply EqDec.eq_dec. Defined.
